src/Iris/Lithium/Islaris/Automation.lean
@@ -1,0 +1,972 @@
+/-
+Copyright (c) 2025 Michael Sammler. All rights reserved.
+Released under Apache 2.0 license as described in the file LICENSE.
+Authors: Michael Sammler
+-/
+import Iris.BI
+import Iris.ProofMode
+import Iris.Lithium.Base
+import Iris.Lithium.Lithium
+import Iris.Lithium.Islaris.Isla
+import Iris.Lithium.Islaris.Instructions.InstrLdr
+import Iris.Lithium.Islaris.Instructions.InstrStr
+
+namespace Islaris
+open Lean Iris BI ProofMode Elab Meta Lithium
+
+variable {PROP : Type u} [BI PROP]
+
+section bitvecCast
+def bitvecCastOkR [BI PROP] {n} (b : BitVec n) (n' : Nat) (E : BitVec n' → PROP) : PROP :=
+  iprop(∃ h : n = n', E (b.cast h))
+
+@[irun_preprocess]
+def bitvecCastOk {n} (b : BitVec n) (n' : Nat) : Li PROP (BitVec n') where
+  run := bitvecCastOkR b n'
+  mono' E1 E2 := by mysorry
+
+theorem bitvecCastOk_tac n (b : BitVec n) P E :
+  (P ⊢ E b) →
+  (P ⊢ bitvecCastOkR (PROP:=PROP) b n E) := by mysorry
+
+@[irun_tac bitvecCastOkR _ _ _]
+def irunBitvecCast : IRunTacticType := fun goal _config => do profileitM Exception "irunBitvecCast" (← getOptions) do
+  let ig := goal
+  let { u, prop, bi, hyp, goal:=G } := ig
+
+  let_expr bitvecCastOkR _ _ n b n' E := G | return none
+  let .true ← isDefEq n n' | return none
+  let g' := IrisGoalShallow.toExpr { ig with goal := Expr.beta E #[b] }
+  let goal' ← mkFreshExprSyntheticOpaqueMVar g'
+  let pf := mkApp7 (.const ``bitvecCastOk_tac [u]) prop bi n b hyp E goal'
+  return .some (pf, [goal'.mvarId!], [])
+
+end bitvecCast
+
+section subst
+partial def substBaseValExpr (v : Expr) (x : VarName) (e : Expr) : MetaM Expr :=
+  match_expr e with
+  | BaseVal.symbolic v' => do
+    let some v' := v'.nat?
+      | throwError "substBaseValExpr: cannot compute substitution in {e}"
+    if v' = x then return v else return e
+  | BaseVal.bool _ => return e
+  | BaseVal.bits _ => return e
+  | BaseVal.enum _ => return e
+  | _ => throwError "substBaseValExpr: cannot compute substitution in {e}"
+
+partial def substValuExpr (v : Expr) (x : VarName) (e : Expr) : MetaM Expr :=
+  match_expr e with
+  | Valu.base v' => do return e.modifyApp1 (← substBaseValExpr v x v')
+  | Valu.i _ _ => do return e
+  | Valu.string _ => do return e
+  | Valu.unit => do return e
+  | Valu.vector vs => do
+    let some vs ← vs.mapMListLit (substValuExpr v x)
+      | throwError "substValuExpr: cannot compute substitution in {e}"
+    return e.modifyApp1 vs
+  | Valu.list vs => do
+    let some vs ← vs.mapMListLit (substValuExpr v x)
+      | throwError "substValuExpr: cannot compute substitution in {e}"
+    return e.modifyApp1 vs
+  | Valu.struct vs => do
+    let some vs ← vs.mapMListLit (λ e =>
+      match_expr e with
+      | Prod.mk _ _ _ v' => do return e.modifyApp1 (← substValuExpr v x v')
+      | _ => throwError "substValuExpr: cannot compute substitution in {e}"
+      )
+      | throwError "substValuExpr: cannot compute substitution in {e}"
+    return e.modifyApp1 vs
+  | Valu.constructor _ v' => do return e.modifyApp1 (← substValuExpr v x v')
+  | Valu.poison => do return e
+  | _ => throwError "substValuExpr: cannot compute substitution in {e}"
+
+partial def substExpExpr (v : Expr) (x : VarName) (e : Expr) : MetaM Expr :=
+  match_expr e with
+  | Exp.val v' => do return e.modifyApp1 (← substBaseValExpr v x v')
+  | Exp.unop _ e1 => do return e.modifyApp1 (← substExpExpr v x e1)
+  | Exp.binop _ e1 e2 => do return e.modifyApp2 (← substExpExpr v x e1) (← substExpExpr v x e2)
+  | Exp.manyop _ es => do
+    let some es ← es.mapMListLit (substExpExpr v x)
+      | throwError "substExpExpr: cannot compute substitution in {e}"
+    return e.modifyApp1 es
+  | Exp.ite e1 e2 e3 => do return mkApp3 (mkConst ``Exp.ite) (← substExpExpr v x e1) (← substExpExpr v x e2) (← substExpExpr v x e3)
+  | _ => throwError "substExpExpr: cannot compute substitution in {e}"
+
+partial def substSmtExpr (v : Expr) (x : VarName) (e : Expr) : MetaM Expr :=
+  -- do logInfo m!"Smt: {e}"
+  match_expr e with
+  | Smt.declareConst _ _ => do return e
+  | Smt.defineConst _ e' => do return e.modifyApp1 (← substExpExpr v x e')
+  | Smt.assert e' => do return e.modifyApp1 (← substExpExpr v x e')
+  | Smt.defineEnum _ _ _ => do return e
+  | _ => throwError "substSmtExpr: cannot compute substitution in {e}"
+
+partial def substEventExpr (v : Expr) (x : VarName) (e : Expr) : MetaM Expr :=
+  -- do logInfo m!"Event: {e}"
+  match_expr e with
+  | Event.smt s => do return e.modifyApp1 (← substSmtExpr v x s)
+  | Event.branch _ _ => do return e
+  | Event.readReg _ _ v' => do return e.modifyApp1 (← substValuExpr v x v')
+  | Event.writeReg _ _ v' => do return e.modifyApp1 (← substValuExpr v x v')
+  | Event.readMem v' rkind addr nb tag => do
+    let some tag ← tag.mapMOptionLit (substValuExpr v x)
+      | throwError "substEventExpr: cannot compute substitution in {e}"
+    return mkApp5 (mkConst ``Event.readMem) (← substValuExpr v x v') (← substValuExpr v x rkind) (← substValuExpr v x addr) nb tag
+  | Event.writeMem v' wkind addr data nb tag => do
+    let some tag ← tag.mapMOptionLit (substValuExpr v x)
+      | throwError "substEventExpr: cannot compute substitution in {e}"
+    return mkApp6 (mkConst ``Event.writeMem) (← substValuExpr v x v') (← substValuExpr v x wkind) (← substValuExpr v x addr) (← substValuExpr v x data) nb tag
+  | Event.branchAddress addr => do return mkApp (mkConst ``Event.branchAddress) (← substValuExpr v x addr)
+  | Event.barrier bkind => do return mkApp (mkConst ``Event.barrier) (← substValuExpr v x bkind)
+  | Event.cacheOp ckind addr => do return mkApp2 (mkConst ``Event.cacheOp) (← substValuExpr v x ckind) (← substValuExpr v x addr)
+  | Event.markReg _ _ => do return e
+  | Event.cycle => do return e
+  | Event.instr opcode => do return mkApp (mkConst ``Event.instr) (← substValuExpr v x opcode)
+  | Event.sleeping _ => do return e
+  | Event.wakeRequest => do return e
+  | Event.sleepRequest => do return e
+  | Event.call _ => do return e
+  | Event.return _ => do return e
+  | Event.assumeReg _ _ v' => do return e.modifyApp1 (← substValuExpr v x v')
+  | Event.assume _ => do return e
+  | Event.funAssume _ v' a => do return e.modifyApp2 (← substValuExpr v x v') a
+  | Event.useFunAssume _ v' a => do return e.modifyApp2 (← substValuExpr v x v') a
+  | Event.abstractCall _ v' a => do return e.modifyApp2 (← substValuExpr v x v') a
+  | Event.abstractPrimop _ v' a => do return e.modifyApp2 (← substValuExpr v x v') a
+  | _ => throwError "substEventExpr: cannot compute substitution in {e}"
+
+
+partial def substTraceExpr (v : Expr) (x : VarName) (e : Expr) : MetaM Expr :=
+  match_expr e with
+  | IslaTrace.nil => return e
+  | IslaTrace.cons e t' => return mkApp2 (mkConst ``IslaTrace.cons) (← substEventExpr v x e) (← substTraceExpr v x t')
+  | IslaTrace.cases ts => do
+    let some ts ← ts.mapMListLit (substTraceExpr v x) | throwError "substTraceExpr: cannot compute substitution in {e}"
+    return mkApp (mkConst ``IslaTrace.cases) ts
+  | _ => throwError "substTraceExpr: cannot compute substitution in {e}"
+-- we could also return [mkApp3 (mkConst ``substTrace) v (mkNatLit x) e], but that would not help
+
+def substTraceOkR (v : BaseVal) (x : VarName) (t : IslaTrace) (E : IslaTrace → PROP) : PROP :=
+  E (substTrace v x t)
+
+@[irun_preprocess]
+def substTraceOk (v : BaseVal) (x : VarName) (t : IslaTrace) : Li PROP IslaTrace := {
+  run := substTraceOkR v x t
+  mono' E1 E2 := by mysorry
+}
+
+@[irun_tac substTraceOkR _ _ _ _]
+def irunSubstTraceOk : IRunTacticType := fun goal _config => do profileitM Exception "irunSubstTraceOk" (← getOptions) do
+  let ig := goal
+  let G := ig.goal
+
+  let_expr substTraceOkR _ v x t E := G | return none
+  let .some x := x.nat? | return none
+  let t' := ← substTraceExpr v x t
+  let g' := {ig with goal := Expr.beta E #[t']}.toExpr
+  let goal' ← mkFreshExprSyntheticOpaqueMVar g'
+  let pf ← mkExpectedTypeHint goal' ig.toExpr
+  return .some (pf, [goal'.mvarId!], [])
+
+end subst
+
+section fns
+
+def expOkR [BI PROP] (e : Exp) (E : BaseVal → PROP) : PROP := sorry
+
+@[irun_preprocess]
+def expOk (e : Exp) : Li PROP BaseVal where
+  run := expOkR e
+  mono' E1 E2 := by mysorry
+
+def aexpOkR [BI PROP] (e : AExp) (E : BaseVal → PROP) : PROP := sorry
+
+@[irun_preprocess]
+def aexpOk (e : AExp) : Li PROP BaseVal where
+  run := aexpOkR e
+  mono' E1 E2 := by mysorry
+
+def asmOkR [BI PROP] (t : IslaTrace) : PROP := sorry
+
+@[irun_preprocess]
+def asmOk (t : IslaTrace) : Li PROP Empty where
+  run _ := asmOkR t
+  mono' E1 E2 := by mysorry
+
+end fns
+
+section regs
+
+def readAccessor (al : AccessorList) (v : Valu) : Option Valu :=
+  match al with
+  | [] => some v
+  | .field f :: al' => do
+    let s ← (match v with | .struct s => some s | _ => none)
+    let v' ← s.find? (λ x => x.1 = f)
+    readAccessor al' v'.2
+
+def readAccessorOkR (al : AccessorList) (v : Valu) (E : Valu → PROP) : PROP :=
+  iprop(∃ v', ⌜readAccessor al v = some v'⌝ ∗ E v')
+
+@[irun_preprocess]
+def readAccessorOk (al : AccessorList) (v : Valu) : Li PROP Valu where
+  run := readAccessorOkR al v
+  mono' E1 E2 := by mysorry
+
+@[irun]
+theorem readAccessorOk_field_eq f v s:
+  readAccessorOkR (PROP:=PROP) [Accessor.field f] (Valu.struct ((f, v) :: s)) :- do return v := by mysorry
+
+@[irun:mid]
+theorem readAccessorOk_field_neq f f' v s:
+  f ≠ f' →
+  readAccessorOkR (PROP:=PROP) [Accessor.field f] (Valu.struct ((f', v) :: s)) :- readAccessorOk [Accessor.field f] (Valu.struct s) := by mysorry
+
+inductive RegKind where
+| reg (re : String)
+| field (re f : String)
+deriving DecidableEq, ToExpr
+
+def _root_.Lean.Expr.regKind? (e : Expr) : Option RegKind :=
+  match_expr e with
+  | RegKind.reg re =>
+    match re with
+    | .lit (Literal.strVal re) => some (.reg re)
+    | _ => none
+  | RegKind.field re f =>
+    match re, f with
+    | .lit (Literal.strVal re), .lit (Literal.strVal f) => some (.field re f)
+    | _, _ => none
+  | _ => none
+
+
+inductive ValuShape where
+| exact (v : Valu)
+| struct (ss : List (String × ValuShape))
+| mask (n : Nat) (mask : Int) (v : Int)
+| bits (n : Nat)
+| prop (P : Valu → Prop)
+| unknown
+
+@[irun_simp, irun_solve]
+def Valu.hasShape : Valu → ValuShape → Prop
+| v, .exact v' => v = v'
+| .struct s, .struct s' => s.length = s'.length -- TODO: missing
+| .base <| .bits _b, .mask _n _m _v' => False -- TODO
+| .base <| .bits b, .bits n => b.size = n
+| v, .prop P => P v
+| _, .unknown => True
+| _, _ => False
+
+partial def lookupRegCol (regs : List (RegKind × ValuShape)) (f : RegKind) : Option ValuShape :=
+-- TODO: lookup in fields of a struct
+  (·.2) <$> (regs.find? (λ (f', _) => if f = f' then true else false))
+
+theorem lookupRegCol_cons_eq regs f f' s :
+  f = f' →
+  lookupRegCol ((f', s)::regs) f = some s := by mysorry
+
+theorem lookupRegCol_cons_neq regs f f' s s':
+  lookupRegCol regs f = some s' →
+  if f ≠ f' then -- uses reduction in the kernel
+    lookupRegCol ((f', s)::regs) f = some s'
+  else
+    True := by mysorry
+
+partial def lookupRegColExpr (regs : Expr) (f : RegKind) : MetaM (Option (Expr × Expr)) :=
+  do
+  match_expr ← whnfR regs with
+  | List.nil _ => return none
+  | List.cons _ p regs' =>
+    match_expr p with
+    | Prod.mk _ _ fe' s =>
+      let some f' := fe'.regKind? | throwError "lookupRegCol: cannot compute regcol lookup in {regs}"
+      if f' == f then
+        return some (s, mkApp5 (mkConst ``lookupRegCol_cons_eq) regs (toExpr f) fe' s
+          (mkApp2 (.const ``Eq.refl [1]) (mkConst ``RegKind) fe'))
+      else
+        let some (s', pf) ← lookupRegColExpr regs' f | return none
+        return some (s', mkApp6 (mkConst ``lookupRegCol_cons_neq) regs (toExpr f) fe' s s' pf)
+    | _ => throwError "lookupRegCol: cannot compute regcol lookup in {regs}"
+  | _ => throwError "lookupRegCol: cannot compute regcol lookup in {regs}"
+
+def lookupRegColOkR (regs : List (RegKind × ValuShape)) (f : RegKind) (E : ValuShape → PROP) : PROP :=
+  iprop(∃ v, ⌜lookupRegCol regs f = some v⌝ ∗ E v)
+
+@[irun_preprocess]
+def lookupRegColOk (regs : List (RegKind × ValuShape)) (f : RegKind) : Li PROP ValuShape where
+  run := lookupRegColOkR regs f
+  mono' E1 E2 := by mysorry
+
+theorem lookupRegColOk_tac regs f s E P :
+  lookupRegCol regs f = some s →
+  (P ⊢ E s) →
+  P ⊢ lookupRegColOkR (PROP:=PROP) regs f E  := by mysorry
+
+@[irun_tac lookupRegColOkR _ _ _]
+def irunLookupRegCol : IRunTacticType := fun goal _config => do profileitM Exception "irunLookupRegCol" (← getOptions) do
+  let ig := goal
+  let { u, prop, bi, hyp, goal:=G } := ig
+
+  let_expr lookupRegColOkR _ _ regs fe E := G | return none
+  let some f := fe.regKind? | return none
+  let some (e, epf) ← lookupRegColExpr regs f | return none
+  let g' := IrisGoalShallow.toExpr { ig with goal := Expr.beta E #[e] }
+  let goal' ← mkFreshExprSyntheticOpaqueMVar g'
+  let pf := mkApp9 (.const ``lookupRegColOk_tac [u]) prop bi regs fe e E hyp epf goal'
+  return .some (pf, [goal'.mvarId!], [])
+
+
+def reg (s : String) : Atom PROP Valu := sorry
+def regField (s : String) (f : String) : Atom PROP Valu := sorry
+def regCol (rs : List (RegKind × ValuShape)) : Atom PROP Unit := sorry
+
+inductive RegPtstoKind where
+| reg (_ : Valu)
+| regCol (_ : List (RegKind × ValuShape))
+
+def regPtsto (s : String) : Atom PROP RegPtstoKind := Atom.mk λ
+  | .reg v => reg s # v
+  | .regCol regs => regCol regs # ()
+
+inductive RegStructPtstoKind where
+| reg (_ : Valu)
+| regCol (_ : List (RegKind × ValuShape))
+
+def regStructPtsto (s : String) (f : String) : Atom PROP RegStructPtstoKind := Atom.mk λ
+  | .reg v => regField s f # v
+  | .regCol regs => regCol regs # ()
+
+@[irun]
+theorem cancel_regPtsto_reg s v :
+  cancelR (PROP:=PROP) (reg s # v) (regPtsto s) :- .pure (.reg v) := by mysorry
+
+@[irun]
+theorem cancel_regStructPtsto_reg s f v :
+  cancelR (PROP:=PROP) (regField s f # v) (regStructPtsto s f) :- .pure (.reg v) := by mysorry
+
+
+theorem cancel_regPtsto_regCol_tac regs s E P :
+  (P ⊢ E (.regCol regs)) →
+  P ⊢ cancelR (PROP:=PROP) (regCol regs # ()) (regPtsto s) E  := by mysorry
+
+theorem cancel_regStructPtsto_regCol_tac regs s f E P :
+  (P ⊢ E (.regCol regs)) →
+  P ⊢ cancelR (PROP:=PROP) (regCol regs # ()) (regStructPtsto s f) E := by mysorry
+
+
+@[irun_tac cancelR (regCol _ # _) (regPtsto _) _, cancelR (regCol _ # _) (regStructPtsto _ _) _]
+def irunCancelRegCol : IRunTacticType := fun goal _config => do profileitM Exception "irunCancelRegCol" (← getOptions) do
+  let ig := goal
+  let { u, prop, bi, hyp, goal:=G } := ig
+
+  let_expr cancelR _ _ _ A A' E := G | return none
+  let_expr Atom.ref _ _ A _ := A | return none
+  let_expr regCol _ regs := A | return none
+  let some (cst, f, pf) := (match_expr A' with
+    | regPtsto _ s =>
+      match s with
+      | .lit (.strVal ss) =>
+        some (``RegPtstoKind.regCol,
+        RegKind.reg ss,
+        mkApp6 (.const ``cancel_regPtsto_regCol_tac [u]) prop bi regs s E hyp)
+      | _ => none
+    | regStructPtsto _ re f =>
+      match re, f with
+      | .lit (.strVal res), .lit (.strVal fs) =>
+        some (``RegStructPtstoKind.regCol,
+        RegKind.field res fs,
+        mkApp7 (.const ``cancel_regStructPtsto_regCol_tac [u]) prop bi regs re f E hyp)
+      | _, _ => none
+    | _ => none) | return none
+  let some _ ← lookupRegColExpr regs f | return none
+  let res := mkApp (mkConst cst) regs
+  let m ← mkFreshExprSyntheticOpaqueMVar <| IrisGoalShallow.toExpr { ig with goal := Expr.beta E #[res] }
+  let pf := mkApp pf m
+  return .some (pf, [m.mvarId!], [])
+
+
+-- @[irun]
+theorem cancel_regPtsto_regCol regs s :
+  .reg s ∈ regs.map (·.1) →
+  cancelR (PROP:=PROP) (regCol regs # ()) (regPtsto s) :- .pure (.regCol regs) := by mysorry
+
+-- @[irun]
+theorem cancel_regStructPtsto_regCol regs s f:
+  .field s f ∈ regs.map (·.1) →
+  cancelR (PROP:=PROP) (regCol regs # ()) (regStructPtsto s f) :- .pure (.regCol regs) := by mysorry
+
+end regs
+
+section spec
+
+inductive Label where
+| readMem (a : BitVec 64) (v : BitVecN)
+| writeMem (a : BitVec 64) (v : BitVecN)
+| instrTrap (pc : BitVec 64)
+
+def Spec : Type := List Label → Prop
+
+def Spec.nil : Spec := λ κs => κs = []
+def Spec.cons (lb : Label) (P : Spec) : Spec := λ κs => κs = [] ∨ ∃ κs', κs' = lb::κs' ∧ (κs' = [] ∨ P κs')
+def Spec.app (ls : List Label) (P : Spec) : Spec := ls.foldr Spec.cons P
+
+
+def specTrace : Atom PROP Spec := sorry
+
+def specConsOkR [BI PROP] (lb : Label) (P : Spec) (E : Spec → PROP) : PROP := sorry
+
+@[irun_preprocess]
+def specConsOk (lb : Label) (P : Spec) : Li PROP Spec where
+  run := specConsOkR lb P
+  mono' E1 E2 := by mysorry
+
+@[irun]
+theorem specConsOk_cons lb P lb' :
+  specConsOkR (PROP:=PROP) lb (Spec.cons lb' P) :- do
+    exhale (prop (lb = lb'))
+    return P := by mysorry
+
+end spec
+
+section mem
+
+def ptsto (a : BitVec 64) (n : Nat) : Atom PROP (BitVec n) := sorry
+def array (a : BitVec 64) (n len : Nat) : Atom PROP (List (BitVec n)) := sorry
+def uninit (a : BitVec 64) (len : Nat) : Atom PROP Unit := sorry
+def mmio (a : BitVec 64) (len : Nat) : Atom PROP Unit := sorry
+
+inductive MemPtstoKind where
+| ptsto (n : Nat) (_ : BitVec n)
+| array (a : BitVec 64) (n len : Nat) (_ : List (BitVec n))
+| uninit (a : BitVec 64) (len : Nat)
+| mmio (a : BitVec 64) (len : Nat)
+
+def memPtsto (a : BitVec 64) : Atom PROP MemPtstoKind := Atom.mk λ
+| .ptsto n v => ptsto a n # v
+| .array a' n len vs => array a' n len # vs
+| .uninit a' len => uninit a' len # ()
+| .mmio a' len => mmio a' len # ()
+
+@[irun:high]
+theorem cancel_ptsto_memPtsto a n v :
+  cancelR (PROP:=PROP) (ptsto a n # v) (memPtsto a) :- .pure (.ptsto n v) := by mysorry
+
+@[irun]
+theorem cancel_ptsto_memPtsto_solve a a' n v :
+  a = a' →
+  cancelR (PROP:=PROP) (ptsto a n # v) (memPtsto a') :- .pure (.ptsto n v) := by mysorry
+
+@[irun]
+theorem cancel_ptsto_ptsto_solve a a' n n' v :
+  a = a' →
+  cancelR (PROP:=PROP) (ptsto a n # v) (ptsto a' n') :- bitvecCastOk v n' := by mysorry
+
+@[irun]
+theorem cancel_mmio_memPtsto_solve a a' n v :
+  a ≤ a' ∧ a' ≤ a + BitVec.ofNat 64 n →
+  cancelR (PROP:=PROP) (mmio a n # v) (memPtsto a') :- .pure (.mmio a n) := by mysorry
+
+end mem
+
+section instr
+
+def instr (a : BitVec 64) : Atom PROP (Option IslaTrace) := sorry
+
+def instrPre'R [BI PROP] (isLater : Bool) (a : BitVec 64) (E : PROP) : PROP := sorry
+
+@[irun_preprocess]
+def instrPre' (isLater : Bool) (a : BitVec 64) (G : Li PROP Empty) : Li PROP Empty where
+  run E := instrPre'R isLater a (G.run E)
+  mono' E1 E2 := by mysorry
+
+abbrev instrPre := @instrPre' PROP _ true
+abbrev instrBody := @instrPre' PROP _ false
+
+def instrPreA (a : BitVec 64) : Atom PROP PROP := Atom.mk λ E => instrPre'R true a E
+
+@[irun]
+theorem dualizing_instr_pre a P E :
+  dualizingR (PROP:=PROP) (λ _ => instrPre'R true a P) E ⊣
+    inhaleR (atom_with_ref (instrPreA a) P) E
+ := by mysorry
+
+
+inductive InstrKind PROP where
+| instr (_ : Option IslaTrace)
+| pre (_ : PROP)
+
+def instrKind (a : BitVec 64) : Atom PROP (InstrKind PROP) := Atom.mk λ
+  | .instr i => instr a # i
+  | .pre P => instrPreA a # P
+
+@[irun]
+theorem instrKind_instr a i :
+  cancelR (PROP:=PROP) (instr a # i) (instrKind a) :- .pure (.instr i) := by mysorry
+
+@[irun:low]
+theorem instrKind_instr_solve a a' i :
+  a = a' →
+  cancelR (PROP:=PROP) (instr a # i) (instrKind a') :- .pure (.instr i) := by mysorry
+
+@[irun]
+theorem instrKind_instrPre a P :
+  cancelR (PROP:=PROP) (instrPreA a # P) (instrKind a) :- .pure (.pre P) := by mysorry
+
+@[irun:low]
+theorem instrKind_instrPre_solve a a' P :
+  a = a' →
+  cancelR (PROP:=PROP) (instrPreA a # P) (instrKind a') :- .pure (.pre P) := by mysorry
+
+@[irun]
+theorem instr_pre_runa la a E :
+  instrPre'R (PROP:=PROP) la a E ⊣ (
+    (exhale (PROP:=PROP) (atom (instrKind a))).bind λ
+    | .instr (some t) =>
+      (dualizing (fromEmpty λ _ => E)).bind λ _ =>
+      (inhale (atom_with_ref (reg "_PC") (.base <| .bits a))).bind λ _ =>
+      asmOk t
+    | .instr (none) => fail "instr_pre instr none"
+    | .pre P =>
+      (dualizing (fromEmpty λ _ => E)).bind λ _ =>
+      fromEmpty (λ _ => P)).go := by mysorry
+
+-- TODO: generalize "_PC" to arch reg
+@[irun]
+theorem asmOk_nil :
+  asmOkR (PROP:=PROP) .nil ⊣ (do
+    let .base (.bits (.fromBitVec _ nPC)) ← exhale (atom (reg "_PC")) | fail "pc register is not bitvector"
+    let nPC ← bitvecCastOk nPC 64
+    (exhale (atom (instrKind (PROP:=PROP) nPC))).bind λ
+    | .instr (some t) => do
+      (inhale (atom_with_ref (reg "_PC") (.base <| .bits nPC)))
+      asmOk t
+    | .instr none => do
+      let P ← exhale (atom specTrace)
+      let _ ← specConsOk (.instrTrap nPC) P
+      done
+    | .pre P =>
+      fromEmpty (λ _ => P)).go := by mysorry
+
+end instr
+
+section exp
+
+def unopOkR [BI PROP] (op : Unop) (v : BaseVal) (E : BaseVal → PROP) : PROP := sorry
+
+@[irun_preprocess]
+def unopOk (op : Unop) (v : BaseVal) : Li PROP BaseVal where
+  run := unopOkR op v
+  mono' E1 E2 := by mysorry
+
+def binopOkR [BI PROP] (op : Binop) (v1 v2 : BaseVal) (E : BaseVal → PROP) : PROP := sorry
+
+@[irun_preprocess]
+def binopOk (op : Binop) (v1 v2 : BaseVal) : Li PROP BaseVal where
+  run := binopOkR op v1 v2
+  mono' E1 E2 := by mysorry
+
+def manyopOkR [BI PROP] (op : Manyop) (vs : List BaseVal) (E : BaseVal → PROP) : PROP := sorry
+
+@[irun_preprocess]
+def manyopOk (op : Manyop) (vs : List BaseVal) : Li PROP BaseVal where
+  run := manyopOkR op vs
+  mono' E1 E2 := by mysorry
+
+
+@[irun]
+theorem unopOk_not b :
+  unopOkR (PROP:=PROP) Unop.not (BaseVal.bool b) :-
+    do return (.bool (¬ b)) := by mysorry
+@[irun]
+theorem unopOk_extract {n} (b : BitVec n) s e :
+  unopOkR (PROP:=PROP) (Unop.extract e s) (BaseVal.bits b) :-
+    do return (.bits (b.extractLsb' s (e + 1 - s))) := by mysorry
+@[irun]
+theorem unopOk_zeroExtend {n} (b : BitVec n) m :
+  unopOkR (PROP:=PROP) (Unop.zeroExtend m) (BaseVal.bits b) :-
+    do return (.bits (b.zeroExtend (m + n))) := by mysorry
+
+@[irun]
+theorem binopOk_eq_bits {n} (b1 b2 : BitVec n) :
+  binopOkR (PROP:=PROP) (Binop.eq) (BaseVal.bits b1) (BaseVal.bits b2) :-
+    do return (.bool (b1 = b2)) := by mysorry
+
+@[irun]
+theorem manyopOk_bvand2 {n} (b1 b2 : BitVec n) :
+  manyopOkR (PROP:=PROP) (Manyop.bvManyArith BvManyArith.bvand) [BaseVal.bits b1, BaseVal.bits b2] :-
+    do return (.bits (b1 &&& b2)) := by mysorry
+@[irun]
+theorem manyopOk_bvor2 {n} (b1 b2 : BitVec n) :
+  manyopOkR (PROP:=PROP) (Manyop.bvManyArith BvManyArith.bvor) [BaseVal.bits b1, BaseVal.bits b2] :-
+    do return (.bits (b1 ||| b2)) := by mysorry
+@[irun]
+theorem manyopOk_bvadd2 {n} (b1 b2 : BitVec n) :
+  manyopOkR (PROP:=PROP) (Manyop.bvManyArith BvManyArith.bvadd) [BaseVal.bits b1, BaseVal.bits b2] :-
+    do return (.bits (b1 + b2)) := by mysorry
+@[irun]
+theorem manyopOk_concat2 {n1 n2} (b1 : BitVec n1) (b2 : BitVec n2) :
+  manyopOkR (PROP:=PROP) (Manyop.concat) [BaseVal.bits b1, BaseVal.bits b2] :-
+    do return (.bits (b1 ++ b2)) := by mysorry
+
+
+@[irun]
+theorem expOk_unop op e :
+  expOkR (PROP:=PROP) (.unop op e) :- (do
+    let v ← expOk e
+    unopOk op v) := by mysorry
+@[irun]
+theorem aexpOk_unop op e :
+  aexpOkR (PROP:=PROP) (.unop op e) :- (do
+    let v ← aexpOk e
+    unopOk op v) := by mysorry
+
+@[irun]
+theorem expOk_binop op e1 e2 :
+  expOkR (PROP:=PROP) (.binop op e1 e2) :- (do
+    let v1 ← expOk e1
+    let v2 ← expOk e2
+    binopOk op v1 v2) := by mysorry
+@[irun]
+theorem aexpOk_binop op e1 e2 :
+  aexpOkR (PROP:=PROP) (.binop op e1 e2) :- (do
+    let v1 ← aexpOk e1
+    let v2 ← aexpOk e2
+    binopOk op v1 v2) := by mysorry
+
+@[irun]
+theorem expOk_manyop2 op e1 e2 :
+  expOkR (PROP:=PROP) (.manyop op [e1, e2]) :- (do
+    let v1 ← expOk e1
+    let v2 ← expOk e2
+    manyopOk op [v1, v2]) := by mysorry
+@[irun]
+theorem aexpOk_manyop2 op e1 e2 :
+  aexpOkR (PROP:=PROP) (.manyop op [e1, e2]) :- (do
+    let v1 ← aexpOk e1
+    let v2 ← aexpOk e2
+    manyopOk op [v1, v2]) := by mysorry
+
+@[irun]
+theorem expOk_val v :
+  expOkR (PROP:=PROP) (.val v) :- (do return v) := by mysorry
+
+@[irun]
+theorem aexpOk_var re :
+  aexpOkR (PROP:=PROP) (.val <| .var re []) :- (do
+    let k ← exhale (atom (regPtsto re))
+    match k with
+    | .reg v'@(.base v) =>
+      inhale (atom_with_ref (reg re) v')
+      return v
+    | .regCol regs =>
+      let s ← lookupRegColOk regs (.reg re)
+      let v : Valu ← all
+      inhale (prop (v.hasShape s))
+      let .base v' := v | fail "variable is not BaseVal"
+      inhale (atom_with_ref (regCol regs) ())
+      return v'
+    | _ => fail "register does not contain not BaseVal") := by mysorry
+
+@[irun]
+theorem aexpOk_bits b :
+  aexpOkR (PROP:=PROP) (.val <| .bits b) :- (do return (.bits b)) := by mysorry
+@[irun]
+theorem aexpOk_bool b :
+  aexpOkR (PROP:=PROP) (.val <| .bool b) :- (do return (.bool b)) := by mysorry
+@[irun]
+theorem aexpOk_enum b :
+  aexpOkR (PROP:=PROP) (.val <| .enum b) :- (do return (.enum b)) := by mysorry
+
+
+end exp
+
+section events
+
+@[irun]
+theorem asmOk_readReg re v t:
+  asmOkR (PROP:=PROP) (.cons (.readReg re [] v) t) ⊣ (do
+   let rk ← exhale (atom (regPtsto re))
+   match rk with
+   | .reg v' =>
+     inhale (prop (v = v'))
+     inhale (atom_with_ref (reg re) v')
+     asmOk t
+   | .regCol regs =>
+     let s ← lookupRegColOk regs (.reg re)
+     inhale (atom_with_ref (regCol regs) ())
+     inhale (prop (v.hasShape s))
+     asmOk t
+     ).go := by mysorry
+
+@[irun]
+theorem asmOk_readReg_struct re v f t:
+  asmOkR (PROP:=PROP) (.cons (.readReg re [.field f] v) t) ⊣ (do
+   let vread ← readAccessorOk [.field f] v
+   let rk ← exhale (atom (regStructPtsto re f))
+   match rk with
+   | .reg v' =>
+     inhale (prop (vread = v'))
+     inhale (atom_with_ref (regField re f) v')
+     asmOk t
+   | .regCol regs =>
+     let s ← lookupRegColOk regs (.field re f)
+     inhale (atom_with_ref (regCol regs) ())
+     inhale (prop (vread.hasShape s))
+     asmOk t
+     ).go := by mysorry
+
+@[irun]
+theorem asmOk_writeReg re v t:
+  asmOkR (PROP:=PROP) (.cons (.writeReg re [] v) t) ⊣ (do
+   let rk ← exhale (atom (regPtsto re))
+   match rk with
+   | .reg _ =>
+     inhale (atom_with_ref (reg re) v)
+     asmOk t
+   | .regCol _regs =>
+     -- TODO
+     fail "asmOK_writeReg regCol"
+     ).go := by mysorry
+
+
+@[irun]
+theorem asmOk_branchAddress a t:
+  asmOkR (PROP:=PROP) (.cons (.branchAddress a) t) ⊣ asmOkR t := by mysorry
+
+@[irun]
+theorem asmOk_branch i s t:
+  asmOkR (PROP:=PROP) (.cons (.branch i s) t) ⊣ asmOkR t := by mysorry
+
+@[irun]
+theorem asmOk_declareConst_bv v b t:
+  asmOkR (PROP:=PROP) (.cons (.smt <| .declareConst v (.bitVec b)) t) ⊣ (do
+   let n : BitVec b ← all
+   asmOk (← substTraceOk (.bits n) v t)
+     ).go := by mysorry
+@[irun]
+theorem asmOk_declareConst_bool v t:
+  asmOkR (PROP:=PROP) (.cons (.smt <| .declareConst v .bool) t) ⊣ (do
+   let n : Bool ← all
+   asmOk (← substTraceOk (.bool n) v t)
+     ).go := by mysorry
+@[irun]
+theorem asmOk_declareConst_enum v i t:
+  asmOkR (PROP:=PROP) (.cons (.smt <| .declareConst v (.enum i)) t) ⊣ (do
+   let n : SailName ← all
+   asmOk (← substTraceOk (.enum n) v t)
+     ).go := by mysorry
+
+@[irun]
+theorem asmOk_defineConst n e t:
+  asmOkR (PROP:=PROP) (.cons (.smt <| .defineConst n e) t) ⊣ (do
+   let v ← expOk e
+   asmOk (← substTraceOk v n t)
+     ).go := by mysorry
+
+
+@[irun]
+theorem asmOk_assert e t:
+  asmOkR (PROP:=PROP) (.cons (.smt (.assert e)) t) ⊣ (do
+    let .bool b ← expOk e | fail "assert does not return bool"
+    inhale (prop (b))
+    asmOk t).go := by mysorry
+
+@[irun]
+theorem asmOk_assume e t:
+  asmOkR (PROP:=PROP) (.cons (.assume e) t) ⊣ (do
+    let v ← aexpOk e
+    exhale (prop (v = BaseVal.bool true))
+    asmOk t).go := by mysorry
+
+@[irun]
+theorem asmOk_assumeReg re v t:
+  asmOkR (PROP:=PROP) (.cons (.assumeReg re [] v) t) ⊣ (do
+   let rk ← exhale (atom (regPtsto re))
+   match rk with
+   | .reg v' =>
+     exhale (prop (v = v'))
+     inhale (atom_with_ref (reg re) v')
+     asmOk t
+   | .regCol regs =>
+     let s ← lookupRegColOk regs (.reg re)
+     exhale (prop (∀ v' : Valu, v'.hasShape s → v' = v))
+     inhale (atom_with_ref (regCol regs) ())
+     asmOk t
+     ).go := by mysorry
+
+@[irun]
+theorem asmOk_assumeRegField re f v t:
+  asmOkR (PROP:=PROP) (.cons (.assumeReg re [.field f] v) t) ⊣ (do
+   let rk ← exhale (atom (regStructPtsto re f))
+   match rk with
+   | .reg v' =>
+     exhale (prop (v = v'))
+     inhale (atom_with_ref (regField re f) v')
+     asmOk t
+   | .regCol regs =>
+     let s ← lookupRegColOk regs (.field re f)
+     exhale (prop (s = ValuShape.exact v))
+     inhale (atom_with_ref (regCol regs) ())
+     asmOk t
+     ).go := by mysorry
+
+@[irun]
+theorem asmOk_readMem {n na} (vread : BitVec n) (a : BitVec na) kind len tag t :
+  asmOkR (PROP:=PROP) (.cons (.readMem (.base <| .bits vread) kind (.base <| .bits a) len tag) t) ⊣ (do
+   exhale (prop (n = 8 * len ∧ len ≠ 0))
+   let a ← bitvecCastOk a 64
+   let rk ← exhale (atom (memPtsto a))
+   match rk with
+   | .ptsto n' v =>
+     let vread ← bitvecCastOk vread n'
+     inhale (prop (vread = v))
+     inhale (atom_with_ref (ptsto a n') v)
+     asmOk t
+   | .array _a' _n _len _vs => fail "readMem array"
+   | .uninit _a' _len => fail "readMem uninit"
+   | .mmio _a' _len => fail "readMem mmio"
+     ).go := by mysorry
+
+@[irun]
+theorem asmOk_writeMem {n na} (vnew : BitVec n) (a : BitVec na) success kind len tag t :
+  asmOkR (PROP:=PROP) (.cons (.writeMem (.base <| .bool success) kind (.base <| .bits a) (.base <| .bits vnew) len tag) t) ⊣ (do
+   exhale (prop (n = 8 * len ∧ len ≠ 0))
+   let a ← bitvecCastOk a 64
+   let rk ← exhale (atom (memPtsto a))
+   match rk with
+   | .ptsto n' _ =>
+     exhale (prop (n' = n))
+     inhale (atom_with_ref (ptsto a n) vnew)
+     asmOk t
+   | .array _a' _n _len _vs => fail "writeMem array"
+   | .uninit _a' _len => fail "writeMem uninit"
+   | .mmio a' len' =>
+     exhale (prop (a' ≤ a ∧ a + len ≤ a' + len'))
+     let Pκs ← exhale (atom (specTrace))
+     let Pκs' ← specConsOk (.writeMem a vnew) Pκs
+     inhale (atom_with_ref specTrace Pκs')
+     asmOk t
+     ).go := by mysorry
+
+
+end events
+
+end Islaris
+
+namespace Islaris.Aarch64
+
+-- instance : Coe BaseVal Valu where
+--   coe := .base
+
+--@[irun_solve]
+abbrev sysRegs : List (RegKind × ValuShape) := [
+  (.reg "SCTLR_EL1" , .exact (.base <| .bits 0x0000000004000002#64 )),
+  (.reg "SCTLR_EL2" , .exact (.base <| .bits 0x0000000004000002#64 )),
+  (.reg "SCR_EL3" , .exact (.base <| .bits 0x00000501#32 )),
+  (.reg "TCR_EL2" , .exact (.base <| .bits 0#64 )),
+  (.reg "HCR_EL2" , .exact (.base <| .bits 0x0000000080000000#64 )),
+  (.reg "CFG_ID_AA64PFR0_EL1_EL0" , .exact (.base <| .bits 1#4 )),
+  (.reg "CFG_ID_AA64PFR0_EL1_EL1" , .exact (.base <| .bits 1#4 )),
+  (.reg "CFG_ID_AA64PFR0_EL1_EL2" , .exact (.base <| .bits 1#4 )),
+  (.reg "CFG_ID_AA64PFR0_EL1_EL3" , .exact (.base <| .bits 1#4 )),
+  (.reg "OSLSR_EL1" , .exact (.base <| .bits 0#32 )),
+  (.reg "OSDLR_EL1" , .exact (.base <| .bits 0#32 )),
+  (.reg "EDSCR" , .exact (.base <| .bits 0#32 )),
+  (.reg "MPIDR_EL1" , .exact (.base <| .bits 0#64 )),
+  (.reg "MDSCR_EL1" , .exact (.base <| .bits 0#32 )),
+  (.reg "MDCR_EL2" , .exact (.base <| .bits 0#32 )),
+  (.reg "MDCR_EL3" , .exact (.base <| .bits 0#32 )),
+  (.field "PSTATE" "SP" , .exact (.base <| .bits 1#1 )),
+  (.field "PSTATE" "EL" , .exact (.base <| .bits 2#2 )),
+  (.field "PSTATE" "nRW" , .exact (.base <| .bits 0#1 )),
+  (.field "PSTATE" "D" , .exact (.base <| .bits 1#1)),
+  (.reg "__isla_monomorphize_writes", .exact (.base <| .bool false)),
+  (.reg "__isla_monomorphize_reads", .exact (.base <| .bool false)),
+  (.reg "__highest_el_aarch32", .exact (.base <| .bool false)),
+  (.reg "__CNTControlBase", .exact (.base <| .bits 0#52)),
+  (.reg "__v85_implemented", .exact (.base <| .bool false)),
+  (.reg "__v84_implemented", .exact (.base <| .bool false)),
+  (.reg "__v83_implemented", .exact (.base <| .bool false)),
+  (.reg "__v82_implemented", .exact (.base <| .bool false)),
+  (.reg "__v81_implemented", .exact (.base <| .bool true)),
+  (.reg "__trickbox_enabled", .exact (.base <| .bool false))
+]
+
+-- example x :
+--   List.find? (fun x : (_ × _) => x.fst == RegKind.reg "HCR_EL2") sysRegs = x := by
+--   unfold sysRegs ; simp?
+
+
+abbrev CNVZRegs : List (RegKind × ValuShape) := [
+  (.field "PSTATE" "C", .bits 1),
+  (.field "PSTATE" "N", .bits 1),
+  (.field "PSTATE" "V", .bits 1),
+  (.field "PSTATE" "Z", .bits 1)
+]
+end Islaris.Aarch64
+
+
+namespace Islaris.InstrTest
+open Lean Iris BI ProofMode Lithium Instructions Aarch64
+
+variable {PROP} [BI PROP]
+
+def ldrSpec (a : BitVec 64) : Li PROP Empty := do
+  exhale (do
+    atom_with_ref (reg "R1") (.base <| .bits 0x0000000000000008#64)
+    let _ ← atom (reg "R0")
+    atom_with_ref (ptsto 0x0000000000000008#64 64) (0x00000000deadbeef#64)
+    atom_with_ref (regCol sysRegs) ())
+  instrPre a (do
+    exhale (do
+      atom_with_ref (reg "R1") (.base <| .bits 0x0000000000000008#64)
+      atom_with_ref (reg "R0") (.base <| .bits 0x00000000deadbeef#64)
+      atom_with_ref (ptsto 0x0000000000000008#64 64) (0x00000000deadbeef#64)
+      atom (regCol sysRegs))
+    done)
+
+-- #eval instr_ldr
+
+--set_option profiler true in
+--set_option trace.profiler true in
+set_option Elab.async false in
+#time example :
+  ⊢ (do
+    inhale (PROP:=PROP) (atom_with_ref (instr 0x0000000010300000#64) (some instr_ldr))
+    instrBody (0x0000000010300000#64) (ldrSpec (0x0000000010300004#64))
+    ).go := by
+  unfold ldrSpec
+  istart
+  simp only [irun_preprocess]
+  irun
+  -- irun +debug 1
+  -- mysorry
+
+def strSpec (a : BitVec 64) : Li PROP Empty := do
+  exhale (do
+    atom_with_ref (reg "R1") (.base <| .bits 0x0000000000000008#64)
+    atom_with_ref (reg "R9") (.base <| .bits 0x00000000cafebabe#64)
+    atom_with_ref (ptsto 0x0000000000000008#64 64) (0x00000000deadbeef#64)
+    atom_with_ref (regCol sysRegs) ())
+  instrPre a (do
+    exhale (do
+      atom_with_ref (reg "R1") (.base <| .bits 0x0000000000000008#64)
+      atom_with_ref (reg "R9") (.base <| .bits 0x00000000cafebabe#64)
+      atom_with_ref (ptsto 0x0000000000000008#64 64) (0x00000000cafebabe#64)
+      atom (regCol sysRegs))
+    done)
+
+set_option Elab.async false in
+#time example :
+  ⊢ (do
+    inhale (PROP:=PROP) (atom_with_ref (instr 0x0000000010300000#64) (some instr_str))
+    instrBody (0x0000000010300000#64) (strSpec (0x0000000010300004#64))
+    ).go := by
+  unfold strSpec
+  istart
+  simp only [irun_preprocess]
+  irun
+  -- irun +debug 1
+  -- mysorry
