src/Iris/Lithium/Islaris/Base.lean
@@ -1,0 +1,9 @@
+/-
+Copyright (c) 2025 Michael Sammler. All rights reserved.
+Released under Apache 2.0 license as described in the file LICENSE.
+Authors: Michael Sammler
+-/
+import Lean
+
+register_simp_attr isla_preprocess
+register_simp_attr isla_regcol_simp
