src/Iris/Lithium/Islaris/Example.lean
@@ -1,0 +1,56 @@
+/-
+Copyright (c) 2025 Michael Sammler. All rights reserved.
+Released under Apache 2.0 license as described in the file LICENSE.
+Authors: Michael Sammler
+-/
+import Iris.BI
+import Iris.ProofMode
+import Iris.Lithium.Base
+import Iris.Lithium.Lithium
+import Iris.Lithium.Islaris.Isla
+import Iris.Lithium.Islaris.Automation
+import Iris.Lithium.Islaris.Instructions.Example.A0
+import Iris.Lithium.Islaris.Instructions.Example.A4
+import Iris.Lithium.Islaris.Instructions.Example.A8
+import Iris.Lithium.Islaris.Instructions.Example.A10
+import Iris.Lithium.Islaris.Instructions.Example.A14
+
+namespace Islaris
+open Lean Iris BI ProofMode Elab Meta Lithium
+open Instructions.Example Aarch64
+
+variable [BI.{u} PROP]
+
+abbrev testStateSpec : Spec :=
+  Spec.cons (.writeMem (0x101f1000#64) (0#64)) $
+  Spec.cons (.instrTrap (0x000000001030000c#64)) $
+  Spec.nil
+
+
+-- set_option profiler true in
+set_option Elab.async false in
+#time example :
+  ⊢ (do
+    inhale (PROP:=PROP) (atom_with_ref (instr 0x0000000010300000#64) (some a0))
+    inhale (atom_with_ref (instr 0x0000000010300004#64) (some a4))
+    inhale (atom_with_ref (instr 0x0000000010300008#64) (some a8))
+    inhale (atom_with_ref (instr 0x000000001030000c#64) none)
+    inhale (atom_with_ref (instr 0x0000000010300010#64) (some a10))
+    inhale (atom_with_ref (instr 0x0000000010300014#64) (some a14))
+
+    inhale (do
+      atom_with_ref (regCol sysRegs) ()
+      atom_with_ref (reg "_PC") (.base <| .bits 0x0000000010300000#64)
+      atom_with_ref (reg "R30") (.poison)
+      atom_with_ref (reg "R1") (.poison)
+      atom_with_ref (reg "R0") (.poison)
+      atom_with_ref (reg "R27") (.base <| .bits 0x101f1000#64)
+      atom_with_ref (reg "R28") (.poison)
+      atom_with_ref (mmio 0x101f1000#64 8) ()
+      atom_with_ref specTrace testStateSpec
+    )
+    asmOk .nil
+    ).go := by
+  istart
+  simp only [irun_preprocess]
+  irun
